theories/store.v
@@ -68,27 +68,27 @@ Implicit Types σ : gmap loc val.
     | Injr "x" =>
         "Diff" "x".𝟙.𝟙.𝟙 "x".𝟙.𝟙.𝟚 "x".𝟙.𝟚 "x".𝟚
     end.
-#[local] Notation "'match:' e0 'with' | 'Root' => e1 | 'Diff' x1 x2 x3 x4 => e2 'end'" :=
-  (descr_match e0 (λ: <>, e1) (λ: x1 x2 x3 x4, e2))%E
-( x1, x2, x3, x4 at level 1,
+#[local] Notation "'match:' e0 'with' | 'Root' => e1 | 'Diff' x1 x2 x3 x4 => e2 'end'" := (
+  (Val descr_match) e0 (Lam BAnon e1) (Lam x1 (Lam x2 (Lam x3 (Lam x4 e2))))
+)(x1, x2, x3, x4 at level 1,
   e0, e1, e2 at level 200,
   format "'[hv' match:  e0  with  '/' '[' |  Root  =>  '/    ' e1 ']'  '/' '[' |  Diff  x1  x2  x3  x4  =>  '/    ' e2  ']' '/' end ']'"
 ) : expr_scope.
-#[local] Notation "'match:' e0 'with' 'Root' => e1 | 'Diff' x1 x2 x3 x4 => e2 'end'" :=
-  (descr_match e0 (λ: <>, e1) (λ: x1 x2 x3 x4, e2))%E
-( x1, x2, x3, x4 at level 1,
+#[local] Notation "'match:' e0 'with' 'Root' => e1 | 'Diff' x1 x2 x3 x4 => e2 'end'" := (
+  (Val descr_match) e0 (Lam BAnon e1) (Lam x1 (Lam x2 (Lam x3 (Lam x4 e2))))
+)(x1, x2, x3, x4 at level 1,
   e0, e1, e2 at level 200,
   only parsing
 ) : expr_scope.
-#[local] Notation "'match::' e0 'with' | 'Root' => e1 | 'Diff' x1 x2 x3 x4 => e2 'end'" :=
-  (descr_match e0 (λ: <>, e1)%V (λ: x1 x2 x3 x4, e2)%V)%E
-( x1, x2, x3, x4 at level 1,
+#[local] Notation "'match::' e0 'with' | 'Root' => e1 | 'Diff' x1 x2 x3 x4 => e2 'end'" := (
+  (Val descr_match) e0 (Val (ValLam BAnon e1)) (Val (ValLam x1 (Lam x2 (Lam x3 (Lam x4 e2)))))
+)(x1, x2, x3, x4 at level 1,
   e0, e1, e2 at level 200,
   format "'[hv' match::  e0  with  '/' '[' |  Root  =>  '/    ' e1 ']'  '/' '[' |  Diff  x1  x2  x3  x4  =>  '/    ' e2  ']' '/' end ']'"
 ) : expr_scope.
-#[local] Notation "'match::' e0 'with' 'Root' => e1 | 'Diff' x1 x2 x3 x4 => e2 'end'" :=
-  (descr_match e0 (λ: <>, e1)%V (λ: x1 x2 x3 x4, e2)%V)%E
-( x1, x2, x3, x4 at level 1,
+#[local] Notation "'match::' e0 'with' 'Root' => e1 | 'Diff' x1 x2 x3 x4 => e2 'end'" := (
+  (Val descr_match) e0 (Val (ValLam BAnon e1)) (Val (ValLam x1 (Lam x2 (Lam x3 (Lam x4 e2)))))
+)(x1, x2, x3, x4 at level 1,
   e0, e1, e2 at level 200,
   only parsing
 ) : expr_scope.
@@ -98,7 +98,7 @@ Implicit Types σ : gmap loc val.
 #[local] Notation "'&&Root'" :=
   ValRoot.
 #[local] Instance pure_descr_match_Root e1 x1 x2 x3 x4 e2 :
-  PureExec True 9
+  PureExec True 11
     (match:: &&Root with Root => e1 | Diff x1 x2 x3 x4 => e2 end)
     e1.
 Proof.
@@ -127,7 +127,7 @@ Proof.
   solve_pure_exec.
 Qed.
 #[local] Instance pure_descr_match_Diff v1 v2 v3 v4 e1 x1 x2 x3 x4 e2 :
-  PureExec True 24
+  PureExec True 26
     (match:: &&Diff v1 v2 v3 v4 with Root => e1 | Diff x1 x2 x3 x4 => e2 end)
     (subst' x1 v1 (subst' x2 v2 (subst' x3 v3 (subst' x4 v4 e2)))).
 Proof.
